added the traces and agent_view function

SecurityNotation/Logic/logic.lean
@@ -11,24 +11,24 @@ import SecurityNotation.Basic.Syntax.Keys
 
 -- def knows (a : Principal) (m : Message) : Prop :=
 -- based on the Dolev-Yao Model
-inductive derives (initial_knowledge : Principal → Message → Prop) : Principal → Message → Prop where
-  | base : ∀ p m, initial_knowledge p m → derives initial_knowledge p m
+inductive Derives (initial_knowledge : Principal → Message → Prop) : Principal → Message → Prop where
+  | base : ∀ p m, initial_knowledge p m → Derives initial_knowledge p m
   --analysis of the message
-  | pair_unpack_l : ∀ p m1 m2, derives initial_knowledge p (Message.pair m1 m2) → derives initial_knowledge p m1
-  | pair_unpack_r : ∀ p m1 m2, derives initial_knowledge p (Message.pair m1 m2) → derives initial_knowledge p m2
-  | decrypt : ∀ p m k, derives initial_knowledge p (Message.enc m k) → derives initial_knowledge p (Message.key k) → derives initial_knowledge p m
+  | pair_unpack_l : ∀ p m1 m2, Derives initial_knowledge p (Message.pair m1 m2) → Derives initial_knowledge p m1
+  | pair_unpack_r : ∀ p m1 m2, Derives initial_knowledge p (Message.pair m1 m2) → Derives initial_knowledge p m2
+  | decrypt : ∀ p m k, Derives initial_knowledge p (Message.enc m k) → Derives initial_knowledge p (Message.key k) → Derives initial_knowledge p m
   --creating a new message
-  | pair_pack : ∀ p m1 m2, derives initial_knowledge p m1 → derives initial_knowledge p m2 → derives initial_knowledge p (Message.pair m1 m2)
-  | encrypt : ∀ p m k, derives initial_knowledge p m → derives initial_knowledge p (Message.key k) → derives initial_knowledge p (Message.enc m k)
+  | pair_pack : ∀ p m1 m2, Derives initial_knowledge p m1 → Derives initial_knowledge p m2 → Derives initial_knowledge p (Message.pair m1 m2)
+  | encrypt : ∀ p m k, Derives initial_knowledge p m → Derives initial_knowledge p (Message.key k) → Derives initial_knowledge p (Message.enc m k)
 
 
 -- this is the static knowledge that everyone knows before messaging
-inductive initial_knowledge (p : Principal) : Message → Prop where
+inductive Initial_knowledge (p : Principal) : Message → Prop where
   -- this states that principal p knows all agents a
-  | knows_agents : ∀ (a : Principal), initial_knowledge p (Message.agent a)
+  | knows_agents : ∀ (a : Principal), Initial_knowledge p (Message.agent a)
   -- this says that if the key is public they they can know it
-  | knows_public_keys : ∀ (k : Key), k.type = keyType.publicKey → initial_knowledge p (Message.key k)
+  | knows_public_keys : ∀ (k : Key), k.type = keyType.publicKey → Initial_knowledge p (Message.key k)
   -- this states that they will know their own private key
-  | knows_own_private_key : ∀ (k: Key), k.type = keyType.privateKey → k.owner = some p → initial_knowledge p (Message.key k)
+  | knows_own_private_key : ∀ (k: Key), k.type = keyType.privateKey → k.owner = some p → Initial_knowledge p (Message.key k)
   -- this states that the principals know of everyone else who holds the key if they know it
-  | held_keys : ∀ (k : Key), p ∈ k.holders → initial_knowledge p (Message.key k)
+  | held_keys : ∀ (k : Key), p ∈ k.holders → Initial_knowledge p (Message.key k)
