SecurityNotation/Basic/Syntax/Events.lean
@@ -1,0 +1,21 @@
+import SecurityNotation.Basic.Syntax.Principal
+import SecurityNotation.Basic.Syntax.Messages
+import SecurityNotation.Basic.Syntax.Keys
+
+inductive Event : Type where
+  | says : Principal → Principal → Message → Event
+  | gets : Principal → Message → Event
+  deriving Repr, DecidableEq
+
+abbrev Trace := List Event
+
+-- adds an event to a list of already existing events
+-- allows us to have a list of events that have occured in in the current space
+def add_event (e : Event) (t : Trace) : Trace := e :: t
+
+def agent_view (p : Principal) (t : Trace) : Trace :=
+  t.filter ( fun e =>
+    match e with
+    | Event.says sender reciever _ => sender = p || reciever = p
+    | Event.gets reciever _ => reciever = p
+  )
